functions for calculating unconditional envC in i1
in case we want to state correctness in terms of them, since the
compiler constructs its tagenv regardless without knowing whether an
exception will be raised in the middle.

compiler/proofs/conLangProofScript.sml
@@ -2573,6 +2573,29 @@ val ALOOKUP_flat_alloc_tags_galloc_tags = prove(
   fs[MAP_FST_galloc_tags] >>
   fs[MEM_MAP,UNCURRY] >> metis_tac[])
 
+val dec_i1_to_envC_def = Define`
+  dec_i1_to_envC d =
+    case d of
+    | Dtype_i1 mn tds => build_tdefs mn tds
+    | Dexn_i1 mn cn ts => bind cn (LENGTH ts, TypeExn (mk_id mn cn)) emp
+    | _ => emp`
+
+val evaluate_dec_i1_to_envC = store_thm("evaluate_dec_i1_to_envC",
+  ``∀ck genv cenv s d res. evaluate_dec_i1 ck genv cenv s d res ⇒
+    ∀v. SND res = Rval v ⇒ dec_i1_to_envC d = FST v``,
+  ho_match_mp_tac evaluate_dec_i1_ind >> simp[dec_i1_to_envC_def])
+
+val decs_i1_to_envC_def = Define`
+  decs_i1_to_envC [] = emp ∧
+  decs_i1_to_envC (d::ds) = merge (decs_i1_to_envC ds) (dec_i1_to_envC d)`
+
+val evaluate_decs_i1_to_envC = store_thm("evaluate_decs_i1_to_envC",
+  ``∀ck genv cenv s ds res. evaluate_decs_i1 ck genv cenv s ds res ⇒
+    ∃envC'. decs_i1_to_envC ds = envC' ++ FST(SND res)∧
+            (SND(SND(SND res)) = NONE ⇒ envC' = [])``,
+  ho_match_mp_tac evaluate_decs_i1_ind >> simp[decs_i1_to_envC_def,emp_def,merge_def] >>
+  rw[] >> imp_res_tac evaluate_dec_i1_to_envC >> fs[] >> rw[])
+
 val decs_to_i2_correct = Q.prove (
 `!ck genv envC s ds r.
   evaluate_decs_i1 ck genv envC s ds r
